Denote $$\mathcal{L}_0 = \left\{ A\subset\mathbb{R}^n :: \lambda^*)A_=\lambda_*(A) < \infty  \right\}$$
All compact sets and all open set with finite measure are in $\mathcal{L}_0$.
\begin{prop}
	$$\lambda_*(A) = \lambda_*(A+x)$$
	$$\lambda^*(A) = \lambda^*(A+x)$$
\end{prop}

\begin{definition}
	For set in $\mathcal{L}_0$, $\lambda(A)=\lambda^*(A)=\lambda_*(A)$.
\end{definition}
\begin{lemma}
	If $A,B \in \mathcal{L}_0$ and $A\cap B = \emptyset$ then $A\cup B \in \mathcal{L}_0$ and 
	$$\lambda(A\cup B) = \lambda(A)+\lambda(B)$$
\end{lemma}
\begin{proof}
	$$\lambda^*(A\cup B) \leq \lambda^*(A)+ \lambda^*(B) = \lambda(A) + \lambda(B) = = \lambda_*(A) + \lambda_*(B) \leq \lambda_*(A\cup B)  \leq \lambda^*(A\cup B) $$
\end{proof}
\begin{theorem}
	$A\subseteq \mathbb{R}^n$ with $\lambda^*(A)<\infty$. $A \in \mathcal{L}_0$ iff for all $\epsilon > 0 $ exists compact $K$ and open $G$, $K\subseteq A \subseteq G$ and $\lambda(G\setminus K) < \epsilon$
	
	
	\begin{proof}
		$\Rightarrow$:
		
		Let  $A \in \mathcal{L}_0$ . We can find compact $K$ and open $G$, $K\subseteq A \subseteq G$ such that
		$$\lambda(G) < \lambda^*(A) +\frac{\epsilon}{2}$$
		$$\lambda(K) > \lambda_*(A) - \frac{\epsilon}{2}$$
		Note that, by lemma
		$$\lambda(G) = \lambda(K) + \lambda(G\setminus K)$$
		$$\lambda(G\setminus K) = \lambda(G) -\lambda(K) < \epsilon$$
		
		
		$\Leftarrow$:
		
		$$\lambda^*(A) \leq \lambda(G) = \lambda(K) + \lambda(G\setminus K) <\lambda(K)+\epsilon \leq \lambda_*(A) +\epsilon $$
		Thus $\lambda^*(A)  = \lambda_*(A) $ and $A \in \mathcal{L}_0$.
	\end{proof}
\begin{coll}
	If $A,B\in \mathcal{L}_0$, then $A\cup B, A\cap B, A\setminus B  \in \mathcal{L}_0$
	\begin{proof}
		First, show that $A\setminus B \in \mathcal{L}_0$.
		Take $K_1\subseteq A\subseteq G_1$ and $K_2 \subseteq A\subseteq G_2$.
		$$\lambda(G_1\setminus K_1) < \frac{\epsilon}{2}$$
		$$\lambda(G_2\setminus K_2) < \frac{\epsilon}{2}$$
		
		Denote $K = K_1\setminus G_2$ and $G = G_1 \setminus K_2$.
		$$K\subseteq A\setminus B \setminus G$$
		$$G\setminus K = (G_1\setminus K_1) \cup (G_2\setminus K_2)$$
		$$\lambda(G\setminus K)  \leq \lambda(G_1\setminus K_1) + \lambda(G_2\setminus K_2) < \epsilon$$
		
		Now
		$$A\cup B = (A\setminus B) \cup B \in \mathcal{L}_0$$
		$$A\cap B = A\setminus (A\setminus B)   \in \mathcal{L}_0$$
	\end{proof}
\end{coll}
\end{theorem}

\begin{theorem}
	Let $\left\{ A_k \right\}$ set in $\mathcal{L}_0$ and $A \bigcup_{k=1}^\infty A_k$ such that $\lambda^*(A) < \infty$ then $A\in \mathcal{L}_0$ and 
	$$\lambda(A) \leq \sum_{k=1}^\infty \lambda(A_k)$$
		In addition, if $A_i\cap A_j = \emptyset$,
		$$\lambda(A) = \sum_{k=1}^\infty \lambda(A_k)$$
	\begin{proof}
		Suppose $\left\{ A_k \right\}$ are disjoint.
		$$\lambda^*(A) \leq \sum_{k=1}^\infty \lambda^*(A_k) = \sum_{k=1}^\infty \lambda_*(A_k) \leq \lambda_*(A)$$
		
		Thus $A\in \mathcal{L}_0$ and
		$$\lambda(A) = \lambda^*(A) =  \sum_{k=1}^\infty \lambda^*(A_k) =  \sum_{k=1}^\infty \lambda(A_k)$$
		
		Now generally, define $$B_1 = A_1 \in \mathcal{L}_0$$
		$$B_2 = A_2 \setminus A_1$$
		and so on:
		$$B_k = A_k \setminus \bigcup_{i=1}^{k-1} A_i \in \mathcal{L}_0 $$
		
		Now $\left\{ B_k \right\} $ are disjoint and $A = \bigcup_{k=1}^\infty A_k = \bigcup_{k=1}^\infty B_k \in \mathcal{L}_0 $. Thus
		$$\lambda(A) = \lambda\qty(\bigcup_{k=1}^\infty A_k)=\lambda\qty(\bigcup_{k=1}^\infty B_k) = \sum_{k=1}^\infty \lambda(B_k) \leq \sum_{k=1}^\infty \lambda(A_k)  $$
	\end{proof}
\end{theorem}
